Code restructuring in PreparedCertificate and ViewChangeMsgsSelectedByPrimary.
PreparedCertificate stores the view it is for and the operationFromPastView instead of taking them from a prototype.
Added well formatted predicate for ViewChangeMsg. ViewChangeMsgsSelectedByPrimary insists on WF to be true for the
selected ViewChangeMsg-s.

messages.dfy
@@ -1,6 +1,8 @@
 include "network.s.dfy"
+include "library/Library.dfy"
 
 module Messages {
+  import Library
   import opened HostIdentifiers
   import Network
 
@@ -9,27 +11,30 @@ module Messages {
 
   datatype ClientOperation = ClientOperation(sender:HostId, timestamp:nat)
 
+  datatype OperationWrapper = Noop | ClientOp(clientOperation: ClientOperation)
+
   function sendersOf(msgs:set<Network.Message<Message>>) : set<HostIdentifiers.HostId> {
     set msg | msg in msgs :: msg.sender
   }
 
-  datatype PreparedCertificate = PreparedCertificate(votes:set<Network.Message<Message>>) {
-    function prototype() : Message 
-      requires |votes| > 0
-    {
-      var prot :| prot in votes;
-      prot.payload
-    }
+  datatype PreparedCertificate = PreparedCertificate(view:ViewNum,
+                                                     operationFromPastView:OperationWrapper,
+                                                     votes:set<Network.Message<Message>>) {
     predicate valid(quorumSize:nat) {
-      || empty()
-      || (&& |votes| == quorumSize
-          && prototype().Prepare?
-          && (forall v | v in votes :: v.payload == prototype()) // messages have to be votes that match eachother by the prototype 
-          && (forall v1, v2 | && v1 in votes
-                              && v2 in votes
-                              && v1 != v2
-                                :: v1.sender != v2.sender) // unique senders
-          )
+      || ( && empty() 
+           && operationFromPastView.Noop? )
+      || ( && |votes| == quorumSize
+           && (forall v1, v2 | && v1 in votes
+                               && v2 in votes
+                               && v1 != v2
+                                 :: v1.sender != v2.sender) // unique senders
+           && (forall v1, v2 | && v1 in votes
+                               && v2 in votes
+                                 :: v1.payload == v2.payload) // messages have to be votes that match eachother
+           && (forall v | v in votes 
+                          :: && v.payload.Prepare?
+                             && view == v.payload.view  
+                             && operationFromPastView == ClientOp(v.payload.clientOp)))
     }
     predicate empty() {
       && |votes| == 0
@@ -39,7 +44,8 @@ module Messages {
   datatype ViewChangeMsgsSelectedByPrimary = ViewChangeMsgsSelectedByPrimary(msgs:set<Network.Message<Message>>) {
     predicate valid(view:ViewNum, quorumSize:nat) {
       && |msgs| > 0
-      && (forall v | v in msgs :: && v.payload.ViewChangeMsg? 
+      && (forall v | v in msgs :: && v.payload.ViewChangeMsg?
+                                  && v.payload.WF()
                                   && v.payload.newView == view) // All the ViewChange messages have to be for the same View. 
       && (forall v1, v2 | && v1 in msgs
                           && v2 in msgs
@@ -55,6 +61,10 @@ module Messages {
                      | Commit(view:ViewNum, seqID:SequenceID, clientOp:ClientOperation)
                      | ClientRequest(clientOp:ClientOperation)
                      | ViewChangeMsg(newView:ViewNum, certificates:imap<SequenceID, PreparedCertificate>) // omitting last stable because we don't have checkpointing yet.
-                     | NewViewMsg(newView:ViewNum, vcMsgs:ViewChangeMsgsSelectedByPrimary)
+                     | NewViewMsg(newView:ViewNum, vcMsgs:ViewChangeMsgsSelectedByPrimary) {
+                       predicate WF() {
+                         && (ViewChangeMsg? ==> Library.FullImap(certificates))
+                       }
+                     }
   // ToDo: ClientReply
 }
